coq/theories/heap_sr.v
@@ -1,18 +1,26 @@
+(* This file presents the heap subject reduction theorem. *)
+
 From mathcomp Require Import ssreflect ssrbool eqtype ssrnat seq.
 From Coq Require Import ssrfun Classical Utf8.
-Require Export AutosubstSsr ARS ptr_step ptr_subst era_sr.
+Require Export AutosubstSsr ARS heap_step heap_subst erasure_sr.
 
 Set Implicit Arguments.
 Unset Strict Implicit.
 Unset Printing Implicit Defensive.
 
-Lemma ptr_srX H1 H2 H H' x y z z' A :
+(* To prove the heap subject reduction theorem, a more general version
+   of the theorem is proven first. heap_srX allows for parts of the heap
+   to remain untouched by reduction. Intuitively, the sub-heaps that 
+   participate in heap reductions are proven to obey subject reduction.
+   Finally, the untouched sub-heaps are merged back together with the
+   sub-heaps that come out of heap reduction. *)
+Lemma heap_srX H1 H2 H H' x y z z' A :
   H1 ; x ~ y ~ z : A -> wr_heap H ->
   H1 ∘ H2 => H -> H ; z ~>> H' ; z' ->
   exists H1' H2' x' y',
     H1' ; x' ~ y' ~ z' : A /\ wr_heap H' /\
     pad H2 H2' /\ H1' ∘ H2' => H' /\ x ~>>* x' /\ y ~>>* y'.
-Proof with eauto 7 using pad, era_type, resolve, merge, free, key, dyn_step.
+Proof with eauto 7 using pad, erasure_type, resolve, merge, lookup, key, program_step.
   move=>{H1 x y z A}[H1 x y z A].
   move e1:(nil)=>Γ. move e2:(nil)=>Δ er.
   elim: er H1 H2 H H' z z' e1 e2=>{Γ Δ x y A}.
@@ -29,7 +37,7 @@ Proof with eauto 7 using pad, era_type, resolve, merge, free, key, dyn_step.
       repeat split...
       { econstructor...
         constructor...
-        apply: resolve_wkU... }
+        apply: resolve_wk1... }
       { constructor...
         have//=nfm':=nf_typing erm.
         have//:=resolve_wr_nfi H8 wr1 nfm'. } }
@@ -40,7 +48,7 @@ Proof with eauto 7 using pad, era_type, resolve, merge, free, key, dyn_step.
       repeat split...
       { econstructor...
         constructor...
-        apply: resolve_wkN... }
+        apply: resolve_wk0... }
       { constructor...
         have//=nfm':=nf_typing erm.
         have//:=resolve_wr_nfi H8 wr1 nfm'. } } }
@@ -56,7 +64,7 @@ Proof with eauto 7 using pad, era_type, resolve, merge, free, key, dyn_step.
       repeat split...
       { econstructor...
         constructor...
-        apply: resolve_wkU... }
+        apply: resolve_wk1... }
       { constructor...
         have//=nfm':=nf_typing erm.
         have//:=resolve_wr_nfi H8 wr1 nfm'. } }
@@ -67,7 +75,7 @@ Proof with eauto 7 using pad, era_type, resolve, merge, free, key, dyn_step.
       repeat split...
       { econstructor...
         constructor...
-        apply: resolve_wkN... }
+        apply: resolve_wk0... }
       { constructor...
         have//=nfm':=nf_typing erm.
         have//:=resolve_wr_nfi H8 wr1 nfm'. } } }
@@ -78,25 +86,25 @@ Proof with eauto 7 using pad, era_type, resolve, merge, free, key, dyn_step.
       exists H1'. exists H2'. exists (App x' n). exists (App y' Box).
       repeat split...
       { apply: (star_hom (App^~ n)) rd1=>x y.
-        apply: dyn_step_appL. }
+        apply: program_step_appL. }
       { apply: (star_hom (App^~ Box)) rd2=>x y.
-        apply: dyn_step_appL. } }
+        apply: program_step_appL. } }
     { inv H9. }
-    { have[H1'[mrg' rs]]:=resolve_free H9 H6 mrg. inv rs.
-      have[A0[n0 e]]:=era_lam0_form erm. subst.
+    { have[H1'[mrg' rs]]:=resolve_lookup H9 H6 mrg. inv rs.
+      have[A0[n0 e]]:=erasure_lam0_form erm. subst.
       exists H1'. exists H2. exists (n0.[n/]). exists (m'0.[Box/]).
       repeat split...
-      { have[ern0 _]:=era_lam0_inv erm.
-        apply: era_esubst0... }
-      { have[ern _]:=era_lam0_inv erm.
-        have wr':=free_wr H9 wr.
+      { have[ern0 _]:=erasure_lam0_inv erm.
+        apply: erasure_esubst0... }
+      { have[ern _]:=erasure_lam0_inv erm.
+        have wr':=lookup_wr H9 wr.
         have[wr1 wr2]:=wr_merge_inv mrg' wr'.
         have[Hx[k mrgx]]:=split_self H1'.
         have[_ wrx]:=wr_merge_inv mrgx wr1.
         apply: resolve_subst...
         constructor.
         constructor... }
-      { apply: free_wr... }
+      { apply: lookup_wr... }
       { apply: star1... }
       { apply: star1... } }
     { have[wr1 wr2]:=wr_merge_inv mrg wr.
@@ -113,9 +121,9 @@ Proof with eauto 7 using pad, era_type, resolve, merge, free, key, dyn_step.
       have//:=resolve_wr_box wr4 H11. } }
   { move=>Γ Δ1 Δ2 Δ A B m m' n n' s mrg1 erm ihm ern ihn H1 H2 H H' z z' e1 e2 rs wr mrg2 st; subst.
     inv mrg1. inv rs; inv st.
-    { have//:=era_box_form ern. }
-    { have//:=era_box_form ern. }
-    { have//:=era_box_form ern. }
+    { have//:=erasure_box_form ern. }
+    { have//:=erasure_box_form ern. }
+    { have//:=erasure_box_form ern. }
     { have[wr1 wr2]:=wr_merge_inv mrg2 wr.
       have[H4[mrg3 mrg4]]:=merge_splitR mrg2 H7.
       have[H1'[H2'[x'[y'[wrx[wr'[pd[mrg5[rd1 rd2]]]]]]]]]:=
@@ -130,9 +138,9 @@ Proof with eauto 7 using pad, era_type, resolve, merge, free, key, dyn_step.
         apply: H8.
         apply: resolve_pad... }
       { apply: (star_hom (App^~ n)) rd1=>x y.
-        apply: dyn_step_appL. }
+        apply: program_step_appL. }
       { apply: (star_hom (App^~ n')) rd2=>x y.
-        apply: dyn_step_appL. } }
+        apply: program_step_appL. } }
     { have[H4[mrg3 mrg4]]:=merge_splitL mrg2 H7.
       have[H1'[H2'[x'[y'[wrx[wr'[pd[mrg5[rd1 rd2]]]]]]]]]:=
         ihn _ _ _ _ _ _ erefl erefl H11 wr (merge_sym mrg4) H13.
@@ -141,48 +149,48 @@ Proof with eauto 7 using pad, era_type, resolve, merge, free, key, dyn_step.
       inv wrx.
       exists Hx. exists H2p. exists (App m x'). exists (App m' y').
       repeat split...
-      { have[t tyP]:=dyn_valid (era_dyn_type erm).
-        have[r[tyB/sort_inj e]]:=sta_pi1_inv tyP. subst.
-        have tyn:=dyn_sta_type (era_dyn_type ern).
-        have//=tyBn:=sta_subst tyB tyn.
-        apply: era_conv.
-        apply: sta_conv_beta.
+      { have[t tyP]:=program_valid (erasure_program_reflect erm).
+        have[r[tyB/sort_inj e]]:=logical_pi1_inv tyP. subst.
+        have tyn:=program_logical_reflect (erasure_program_reflect ern).
+        have//=tyBn:=logical_subst tyB tyn.
+        apply: erasure_conv.
+        apply: logical_conv_beta.
         apply: conv_sym.
         apply: star_conv.
-        apply: dyn_sta_red...
+        apply: program_logical_red...
         econstructor...
         apply: tyBn. }
       { econstructor...
         apply: resolve_pad... }
       { apply: (star_hom (App m)) rd1=>x y.
-        apply: dyn_step_appR. }
+        apply: program_step_appR. }
       { apply: (star_hom (App m')) rd2=>x y.
-        apply: dyn_step_appR. } }
+        apply: program_step_appR. } }
     { have[Hx[mrg3 mrg4]]:=merge_splitR mrg2 H7.
-      have[Hy[mrg5 rs]]:=resolve_free H13 H10 (merge_sym mrg4). inv rs.
-      have[A0[n1 e]]:=era_lam0_form erm. subst.
-      exfalso. apply: sta_lam0_pi1_false... }
+      have[Hy[mrg5 rs]]:=resolve_lookup H13 H10 (merge_sym mrg4). inv rs.
+      have[A0[n1 e]]:=erasure_lam0_form erm. subst.
+      exfalso. apply: logical_lam0_pi1_false... }
     { have[H4[mrg3 mrg4]]:=merge_splitR mrg2 H7.
-      have[H5[mrg rs]]:=resolve_free H13 H10 (merge_sym mrg4). inv rs.
+      have[H5[mrg rs]]:=resolve_lookup H13 H10 (merge_sym mrg4). inv rs.
       have[Hx[mrg5 mrg6]]:=merge_splitL (merge_sym mrg) mrg3.
-      have[A0[n0 e]]:=era_lam1_form erm. subst.
-      have[r[ern0 _]]:=era_lam1_inv erm.
-      have wr':=free_wr H13 wr.
+      have[A0[n0 e]]:=erasure_lam1_form erm. subst.
+      have[r[ern0 _]]:=erasure_lam1_inv erm.
+      have wr':=lookup_wr H13 wr.
       have[wr1 wr2]:=wr_merge_inv mrg wr'.
       have[wr3 wr4]:=wr_merge_inv mrg3 wr2.
       have[H3'[k mrg']]:=split_self H3.
       have[_ wr3']:=wr_merge_inv mrg' wr3.
       have vl':=wr_resolve_ptr wr3 H11.
-      have vl:=era_dyn_val ern vl'.
+      have vl:=erasure_program_val ern vl'.
       exists Hx. exists H2. exists n0.[n/]. exists m'0.[n'/].
       repeat split...
-      { apply: era_subst1.
+      { apply: erasure_subst1.
         apply: key_nil.
         apply: merge_nil.
         apply: ern0.
         apply: ern. }
-      { have wf:=dyn_type_wf (era_dyn_type ern0). inv wf.
-        have k1:=resolution (Ptr_well_resolved ern H11) H17 vl' wr3.
+      { have wf:=program_type_wf (erasure_program_reflect ern0). inv wf.
+        have k1:=resolution_stability (Heap_well_resolved ern H11) H17 vl' wr3.
         destruct r.
         { apply: resolve_subst.
           apply: ern0.
@@ -201,28 +209,28 @@ Proof with eauto 7 using pad, era_type, resolve, merge, free, key, dyn_step.
           apply: merge_sym...
           all: eauto.
           constructor... } }
-      { apply: star1. apply: dyn_step_beta1... }
-      { apply: star1. apply: dyn_step_beta1... } } }
+      { apply: star1. apply: program_step_beta1... }
+      { apply: star1. apply: program_step_beta1... } } }
   { move=>Γ Δ A B m m' n t tyS erm ihm tyn H1 H2 H H' z z' e1 e2 rs wr mrg st; subst.
     inv rs; inv st.
     { have[H1'[H2'[x'[y'[wrx[wr'[pd[mrg'[rd1 rd2]]]]]]]]]:=ihm _ _ _ _ _ _ erefl erefl H6 wr mrg H9.
       inv wrx.
       exists H1'. exists H2'. exists (Pair0 x' n t). exists (Pair0 y' Box t).
       repeat split...
-      { have[s[r[ord[tyA[tyB _]]]]]:=sta_sig0_inv tyS.
-        have tyx:=dyn_sta_type (dyn_rd (era_dyn_type erm) rd1).
-        have//=tyBx:=sta_subst tyB tyx.
+      { have[s[r[ord[tyA[tyB _]]]]]:=logical_sig0_inv tyS.
+        have tyx:=program_logical_reflect (program_rd (erasure_program_reflect erm) rd1).
+        have//=tyBx:=logical_subst tyB tyx.
         constructor...
-        apply: sta_conv.
-        apply: sta_conv_beta.
+        apply: logical_conv.
+        apply: logical_conv_beta.
         apply: star_conv.
-        apply: (dyn_sta_red (dyn_sta_type (era_dyn_type erm)))...
+        apply: (program_logical_red (program_logical_reflect (erasure_program_reflect erm)))...
         apply: tyn.
         apply: tyBx. }
       { apply: (star_hom ((Pair0^~ n)^~ t)) rd1=>x y.
-        apply: dyn_step_pair0L. }
+        apply: program_step_pair0L. }
       { apply: (star_hom ((Pair0^~ Box)^~ t)) rd2=>x y.
-        apply: dyn_step_pair0L. } }
+        apply: program_step_pair0L. } }
     { have[e1 e2]:=merge_size mrg. destruct t.
       { exists (Pair0 (Ptr lm) Box U :U H1).
         exists (Pair0 (Ptr lm) Box U :U H2).
@@ -232,7 +240,7 @@ Proof with eauto 7 using pad, era_type, resolve, merge, free, key, dyn_step.
         { econstructor.
           constructor...
           constructor.
-          apply: resolve_wkU... }
+          apply: resolve_wk1... }
         { constructor... } }
       { exists (Pair0 (Ptr lm) Box L :L H1).
         exists (_: H2).
@@ -242,10 +250,10 @@ Proof with eauto 7 using pad, era_type, resolve, merge, free, key, dyn_step.
         { econstructor.
           constructor...
           constructor.
-          apply: resolve_wkN... }
+          apply: resolve_wk0... }
         { constructor... } } } }
   { move=>Γ Δ1 Δ2 Δ A B m m' n n' t mrg1 tyS erm ihm ern ihn H1 H2 H H' z z' e1 e2 rs wr mrg2 st; subst.
-    have[s[r[ord1[ord2[tyA[tyB _]]]]]]:=sta_sig1_inv tyS. inv mrg1. inv rs; inv st.
+    have[s[r[ord1[ord2[tyA[tyB _]]]]]]:=logical_sig1_inv tyS. inv mrg1. inv rs; inv st.
     { have[H4[mrg3 mrg4]]:=merge_splitR mrg2 H10.
       have[H1'[H2'[x'[y'[wrx[wr'[pd[mrg'[rd1 rd2]]]]]]]]]:=
         ihm _ _ _ _ _ _ erefl erefl H11 wr (merge_sym mrg4) H14. inv wrx.
@@ -253,13 +261,13 @@ Proof with eauto 7 using pad, era_type, resolve, merge, free, key, dyn_step.
       have[Hx[mrp1 mrp2]]:=merge_splitL (merge_sym mrg') mrp.
       exists Hx. exists H2p. exists (Pair1 x' n t). exists (Pair1 y' n' t).
       repeat split...
-      { have tyx:=dyn_sta_type (dyn_rd (era_dyn_type erm) rd1).
-        have//=tyBx:=sta_subst tyB tyx.
+      { have tyx:=program_logical_reflect (program_rd (erasure_program_reflect erm) rd1).
+        have//=tyBx:=logical_subst tyB tyx.
         econstructor...
-        apply: era_conv.
-        apply: sta_conv_beta.
+        apply: erasure_conv.
+        apply: logical_conv_beta.
         apply: star_conv.
-        apply: (dyn_sta_red (dyn_sta_type (era_dyn_type erm)))...
+        apply: (program_logical_red (program_logical_reflect (erasure_program_reflect erm)))...
         apply: ern.
         apply: tyBx. }
       { econstructor.
@@ -267,9 +275,9 @@ Proof with eauto 7 using pad, era_type, resolve, merge, free, key, dyn_step.
         apply: H7.
         apply: resolve_pad... }
       { apply: (star_hom ((Pair1^~ n)^~ t)) rd1=>x y.
-        apply: dyn_step_pair1L. }
+        apply: program_step_pair1L. }
       { apply: (star_hom ((Pair1^~ n')^~ t)) rd2=>x y.
-        apply: dyn_step_pair1L. } }
+        apply: program_step_pair1L. } }
     { have[H4[mrg3 mrg4]]:=merge_splitL mrg2 H10.
       have[H1'[H2'[x'[y'[wrx[wr'[pd[mrg'[rd1 rd2]]]]]]]]]:=
         ihn _ _ _ _ _ _ erefl erefl H12 wr (merge_sym mrg4) H14. inv wrx.
@@ -280,9 +288,9 @@ Proof with eauto 7 using pad, era_type, resolve, merge, free, key, dyn_step.
       { econstructor...
         apply: resolve_pad... }
       { apply: (star_hom (Pair1 m^~ t)) rd1=>x y.
-        apply: dyn_step_pair1R. }
+        apply: program_step_pair1R. }
       { apply: (star_hom (Pair1 m'^~ t)) rd2=>x y.
-        apply: dyn_step_pair1R. } }
+        apply: program_step_pair1R. } }
     { have[e1 e2]:=merge_size mrg2. destruct t.
       { exists (Pair1 (Ptr lm) (Ptr ln) U :U H1).
         exists (Pair1 (Ptr lm) (Ptr ln) U :U H2).
@@ -292,8 +300,8 @@ Proof with eauto 7 using pad, era_type, resolve, merge, free, key, dyn_step.
         { econstructor.
           constructor...
           econstructor...
-          apply: resolve_wkU...
-          apply: resolve_wkU... }
+          apply: resolve_wk1...
+          apply: resolve_wk1... }
         { constructor... } }
       { exists (Pair1 (Ptr lm) (Ptr ln) L :L H1).
         exists (_: H2).
@@ -303,8 +311,8 @@ Proof with eauto 7 using pad, era_type, resolve, merge, free, key, dyn_step.
         { econstructor.
           constructor...
           econstructor...
-          apply: resolve_wkN...
-          apply: resolve_wkN... }
+          apply: resolve_wk0...
+          apply: resolve_wk0... }
         { constructor... } } } }
   { move=>Γ Δ1 Δ2 Δ A B C m m' n n' s r t mrg1 tyC
       erm ihm ern _ H1 H2 H H' z z' e1 e2 rs wr mrg2 st; subst.
@@ -316,41 +324,41 @@ Proof with eauto 7 using pad, era_type, resolve, merge, free, key, dyn_step.
       have[Hx[mrp1 mrp2]]:=merge_splitL (merge_sym mrg') mrp.
       exists Hx. exists H2p. exists (LetIn C x' n). exists (LetIn Box y' n').
       repeat split...
-      { apply: era_conv.
-        apply: sta_conv_beta.
+      { apply: erasure_conv.
+        apply: logical_conv_beta.
         apply: conv_sym.
         apply: star_conv.
-        apply: dyn_sta_red...
-        apply: era_letin0...
-        apply: sta_esubst...
+        apply: program_logical_red...
+        apply: erasure_letin0...
+        apply: logical_esubst...
         autosubst. }
       { econstructor.
         apply: merge_sym...
         apply: H8.
         apply: resolve_pad... }
       { apply: (star_hom (LetIn C^~ n)) rd1=>x y.
-        apply: dyn_step_letinL. }
+        apply: program_step_letinL. }
       { apply: (star_hom (LetIn Box^~ n')) rd2=>x y.
-        apply: dyn_step_letinL. } }
+        apply: program_step_letinL. } }
     { have[H4[mrg3 mrg4]]:=merge_splitR mrg2 H7.
-      have[H1'[mrg' rs]]:=resolve_free H13 H10 (merge_sym mrg4). inv rs.
+      have[H1'[mrg' rs]]:=resolve_lookup H13 H10 (merge_sym mrg4). inv rs.
       have[Hx[mrg5 mrg6]]:=merge_splitL (merge_sym mrg') mrg3.
-      have[m1[m2 e]]:=era_pair0_form erm. subst.
-      have[e[_[erm1 tym2]]]:=era_pair0_inv erm. subst.
-      have wr':=free_wr H13 wr.
+      have[m1[m2 e]]:=erasure_pair0_form erm. subst.
+      have[e[_[erm1 tym2]]]:=erasure_pair0_inv erm. subst.
+      have wr':=lookup_wr H13 wr.
       have[wr1 wr2]:=wr_merge_inv mrg2 wr.
       have[wr3 wr4]:=wr_merge_inv H7 wr1.
       have[wr5 wr6]:=wr_merge_inv mrg' wr'.
       have vl:=wr_resolve_ptr wr5 H15.
-      have wf:=dyn_type_wf (era_dyn_type ern). inv wf.  inv H9.
-      have k1:=resolution (Ptr_well_resolved erm1 H15) H17 vl wr5.
+      have wf:=program_type_wf (erasure_program_reflect ern). inv wf.  inv H9.
+      have k1:=resolution_stability (Heap_well_resolved erm1 H15) H17 vl wr5.
       have[H2'[k mrg2']]:=split_self H1'.
       have[_ wr7]:=wr_merge_inv mrg2' wr5.
       exists Hx. exists H2. exists n.[m2,m1/]. exists (n'.[Box,m'0/]).
       repeat split...
       { replace C.[Pair0 m1 m2 t/] with
           C.[Pair0 (Var 1) (Var 0) t .: ren (+2)].[m2,m1/] by autosubst.
-        apply: era_substitution.
+        apply: erasure_substitution.
         apply: ern.
         constructor.
         econstructor.
@@ -373,14 +381,14 @@ Proof with eauto 7 using pad, era_type, resolve, merge, free, key, dyn_step.
       { apply: star1.
         constructor.
         constructor.
-        apply: era_dyn_val... }
+        apply: erasure_program_val... }
       { apply: star1.
         constructor.
         constructor... } }
     { have[H4[mrg3 mrg4]]:=merge_splitR mrg2 H7.
-      have[H1'[mrg' rs]]:=resolve_free H13 H10 (merge_sym mrg4). inv rs.
-      have[m1[m2 e]]:=era_pair1_form erm. subst.
-      exfalso. apply: sta_pair1_sig0_false... } }
+      have[H1'[mrg' rs]]:=resolve_lookup H13 H10 (merge_sym mrg4). inv rs.
+      have[m1[m2 e]]:=erasure_pair1_form erm. subst.
+      exfalso. apply: logical_pair1_sig0_false... } }
   { move=>Γ Δ1 Δ2 Δ A B C m m' n n' s r1 r2 t mrg1 tyC
       erm ihm ern _ H1 H2 H H' z z' e1 e2 rs wr mrg2 st; subst.
     inv mrg1. inv rs; inv st.
@@ -391,42 +399,42 @@ Proof with eauto 7 using pad, era_type, resolve, merge, free, key, dyn_step.
       have[Hx[mrp1 mrp2]]:=merge_splitL (merge_sym mrg') mrp.
       exists Hx. exists H2p. exists (LetIn C x' n). exists (LetIn Box y' n').
       repeat split...
-      { apply: era_conv.
-        apply: sta_conv_beta.
+      { apply: erasure_conv.
+        apply: logical_conv_beta.
         apply: conv_sym.
         apply: star_conv.
-        apply: dyn_sta_red...
-        apply: era_letin1...
-        apply: sta_esubst...
+        apply: program_logical_red...
+        apply: erasure_letin1...
+        apply: logical_esubst...
         autosubst. }
       { econstructor.
         apply: merge_sym...
         apply: H8.
         apply: resolve_pad... }
       { apply: (star_hom (LetIn C^~ n)) rd1=>x y.
-        apply: dyn_step_letinL. }
+        apply: program_step_letinL. }
       { apply: (star_hom (LetIn Box^~ n')) rd2=>x y.
-        apply: dyn_step_letinL. } }
+        apply: program_step_letinL. } }
     { have[H4[mrg3 mrg4]]:=merge_splitR mrg2 H7.
-      have[H1'[mrg' rs]]:=resolve_free H13 H10 (merge_sym mrg4). inv rs.
-      have[m1[m2 e]]:=era_pair0_form erm. subst.
-      exfalso. apply: sta_pair0_sig1_false... }
+      have[H1'[mrg' rs]]:=resolve_lookup H13 H10 (merge_sym mrg4). inv rs.
+      have[m1[m2 e]]:=erasure_pair0_form erm. subst.
+      exfalso. apply: logical_pair0_sig1_false... }
     { have[H4[mrg3 mrg4]]:=merge_splitR mrg2 H7.
-      have[H1'[mrg' rs]]:=resolve_free H13 H10 (merge_sym mrg4). inv rs.
+      have[H1'[mrg' rs]]:=resolve_lookup H13 H10 (merge_sym mrg4). inv rs.
       have[Hx[mrg5 mrg6]]:=merge_splitL (merge_sym mrg') mrg3.
-      have[m1[m2 e]]:=era_pair1_form erm. subst.
-      have[Δ1[Δ2[mrg[e[erm1 erm2]]]]]:=era_pair1_inv erm. inv mrg; subst.
-      have wr':=free_wr H13 wr.
+      have[m1[m2 e]]:=erasure_pair1_form erm. subst.
+      have[Δ1[Δ2[mrg[e[erm1 erm2]]]]]:=erasure_pair1_inv erm. inv mrg; subst.
+      have wr':=lookup_wr H13 wr.
       have[wr1 wr2]:=wr_merge_inv mrg2 wr.
       have[wr3 wr4]:=wr_merge_inv H7 wr1.
       have[wr5 wr6]:=wr_merge_inv mrg' wr'.
       have[wr7 wr8]:=wr_merge_inv H16 wr5.
       have vm:=wr_resolve_ptr wr7 H18.
       have vn:=wr_resolve_ptr wr8 H19.
-      have wf:=dyn_type_wf (era_dyn_type ern). inv wf.  inv H14.
-      have k1:=resolution (Ptr_well_resolved erm1 H18) H21 vm wr7.
-      have//=tyBm1:=sta_subst H17 (dyn_sta_type (era_dyn_type erm1)).
-      have k2:=resolution (Ptr_well_resolved erm2 H19) tyBm1 vn wr8.
+      have wf:=program_type_wf (erasure_program_reflect ern). inv wf.  inv H14.
+      have k1:=resolution_stability (Heap_well_resolved erm1 H18) H21 vm wr7.
+      have//=tyBm1:=logical_subst H17 (program_logical_reflect (erasure_program_reflect erm1)).
+      have k2:=resolution_stability (Heap_well_resolved erm2 H19) tyBm1 vn wr8.
       have[H5'[k5 mrg5']]:=split_self H5.
       have[H6'[k6 mrg6']]:=split_self H6.
       have[_ wr5']:=wr_merge_inv mrg5' wr7.
@@ -435,7 +443,7 @@ Proof with eauto 7 using pad, era_type, resolve, merge, free, key, dyn_step.
       repeat split...
       { replace C.[Pair1 m1 m2 t/] with
           C.[Pair1 (Var 1) (Var 0) t .: ren (+2)].[m2,m1/] by autosubst.
-        apply: era_substitution.
+        apply: erasure_substitution.
         apply: ern.
         econstructor. apply: key_nil.
         constructor.
@@ -470,8 +478,8 @@ Proof with eauto 7 using pad, era_type, resolve, merge, free, key, dyn_step.
       { apply: star1.
         constructor.
         constructor.
-        apply: era_dyn_val...
-        apply: era_dyn_val... }
+        apply: erasure_program_val...
+        apply: erasure_program_val... }
       { apply: star1.
         constructor.
         constructor... } } }
@@ -487,8 +495,8 @@ Proof with eauto 7 using pad, era_type, resolve, merge, free, key, dyn_step.
       repeat split...
       { econstructor...
         constructor...
-        apply: resolve_wkU...
-        apply: resolve_wkU... }
+        apply: resolve_wk1...
+        apply: resolve_wk1... }
       { have//=nfm':=nf_typing erm.
         have//=nfn':=nf_typing ern.
         constructor...
@@ -501,8 +509,8 @@ Proof with eauto 7 using pad, era_type, resolve, merge, free, key, dyn_step.
       repeat split...
       { econstructor...
         constructor...
-        apply: resolve_wkN...
-        apply: resolve_wkN... }
+        apply: resolve_wk0...
+        apply: resolve_wk0... }
       { have//=nfm':=nf_typing erm.
         have//=nfn':=nf_typing ern.
         constructor...
@@ -515,19 +523,19 @@ Proof with eauto 7 using pad, era_type, resolve, merge, free, key, dyn_step.
       exists H1'. exists H2'. exists (Fst x'). exists (Fst y').
       repeat split...
       { apply: (star_hom Fst) rd1=>x y.
-        apply: dyn_step_fst. }
+        apply: program_step_fst. }
       { apply: (star_hom Fst) rd2=>x y.
-        apply: dyn_step_fst. } }
-    { have[H2'[mrg' rs]]:=resolve_free H5 H6 mrg. inv rs.
-      have[m1[m2 e]]:=era_apair_form erm. subst.
-      have[e[erm1 erm2]]:=era_apair_inv erm. subst.
-      have wr':=free_wr H5 wr.
+        apply: program_step_fst. } }
+    { have[H2'[mrg' rs]]:=resolve_lookup H5 H6 mrg. inv rs.
+      have[m1[m2 e]]:=erasure_apair_form erm. subst.
+      have[e[erm1 erm2]]:=erasure_apair_inv erm. subst.
+      have wr':=lookup_wr H5 wr.
       exists H2'. exists H2. exists m1. exists m'0.
       repeat split...
       { apply: star1.
-        apply: dyn_step_proj1. }
+        apply: program_step_proj1. }
       { apply: star1.
-        apply: dyn_step_proj1. } } }
+        apply: program_step_proj1. } } }
   { move=>Γ Δ A B m m' t erm ihm H1 H2 H H' z z' e1 e2 rs wr mrg st; subst.
     inv rs; inv st.
     { have[H1'[H2'[x'[y'[wrx[wr'[pd[mrg'[rd1 rd2]]]]]]]]]:=
@@ -535,47 +543,47 @@ Proof with eauto 7 using pad, era_type, resolve, merge, free, key, dyn_step.
       exists H1'. exists H2'. exists (Snd x'). exists (Snd y').
       repeat split...
       { apply: (star_hom Snd) rd1=>x y.
-        apply: dyn_step_snd. }
+        apply: program_step_snd. }
       { apply: (star_hom Snd) rd2=>x y.
-        apply: dyn_step_snd. } }
-    { have[H2'[mrg' rs]]:=resolve_free H5 H6 mrg. inv rs.
-      have[n1[n2 e]]:=era_apair_form erm. subst.
-      have[e[ern1 ern2]]:=era_apair_inv erm. subst.
-      have wr':=free_wr H5 wr.
+        apply: program_step_snd. } }
+    { have[H2'[mrg' rs]]:=resolve_lookup H5 H6 mrg. inv rs.
+      have[n1[n2 e]]:=erasure_apair_form erm. subst.
+      have[e[ern1 ern2]]:=erasure_apair_inv erm. subst.
+      have wr':=lookup_wr H5 wr.
       exists H2'. exists H2. exists n2. exists n'.
       repeat split...
       { apply: star1.
-        apply: dyn_step_proj2. }
+        apply: program_step_proj2. }
       { apply: star1.
-        apply: dyn_step_proj2. } } }
+        apply: program_step_proj2. } } }
   { move=>Γ Δ A B x x' P m n s tyB erx ihx tyP H1 H2 H H' z z' e1 e2 rs wr mrg st; subst.
     inv rs; inv st.
     exists H1. exists H2. exists x. exists x'.
     repeat split...
-    { have[P0[rdP vlP]]:=sta_vn tyP.
-      have tyP0:=sta_rd tyP rdP.
-      have[n0 e]:=sta_id_canonical tyP0 (convR _ _) vlP. subst.
-      have tyr:=sta_rd tyP rdP.
-      have[r tyI]:=sta_valid tyP.
-      have[tym[tyn/sort_inj e]]:=sta_id_inv tyI. subst.
-      have[tym0[eq1 eq2]]:=sta_refl_inv tyr.
+    { have[P0[rdP vlP]]:=logical_vn tyP.
+      have tyP0:=logical_rd tyP rdP.
+      have[n0 e]:=logical_id_canonical tyP0 (convR _ _) vlP. subst.
+      have tyr:=logical_rd tyP rdP.
+      have[r tyI]:=logical_valid tyP.
+      have[tym[tyn/sort_inj e]]:=logical_id_inv tyI. subst.
+      have[tym0[eq1 eq2]]:=logical_refl_inv tyr.
       have sc:sconv (Refl m .: m .: ids) (P .: n .: ids).
       { move=>[|[|]]//=.
-        apply: conv_trans. apply: sta_conv_refl. apply: conv_sym...
+        apply: conv_trans. apply: logical_conv_refl. apply: conv_sym...
         apply: conv_sym. apply: star_conv...
         apply: conv_trans. apply: conv_sym... eauto. }
       have wkB:nil ⊢ B.[P,n/] : Sort s.
       { replace (Sort s) with (Sort s).[P,n/] by eauto.
-        apply: sta_substitution...
+        apply: logical_substitution...
         repeat constructor...
         all: asimpl... }
-      apply: era_conv.
-      apply: sta_conv_compat sc.
+      apply: erasure_conv.
+      apply: logical_conv_compat sc.
       all: eauto. }
     { apply: star1.
-      apply: dyn_step_rwE. }
+      apply: program_step_rwE. }
     { apply: star1.
-      apply: dyn_step_rwE. } }
+      apply: program_step_rwE. } }
   { move=>Γ Δ A B m m' s eq erm ihm tyB H1 H2 H H' z z' e1 e2 rs wr mrg st; subst.
     have[H1'[H2'[x'[y'[wrx[wr'[pd[mrg'[rd1 rd2]]]]]]]]]:=
       ihm _ _ _ _ _ _ erefl erefl rs wr mrg st. inv wrx.
@@ -583,14 +591,15 @@ Proof with eauto 7 using pad, era_type, resolve, merge, free, key, dyn_step.
     repeat split... }
 Qed.
 
-Theorem ptr_sr H H' x y z z' A :
+(* Theorem 14 (Heap Subject Reduction) *)
+Theorem heap_sr H H' x y z z' A :
   H ; x ~ y ~ z : A -> wr_heap H ->
   H ; z ~>> H' ; z' ->
   exists x' y', H' ; x' ~ y' ~ z' : A /\ wr_heap H' /\ x ~>>* x' /\ y ~>>* y'.
 Proof with eauto.
   move=>wrx wr st.
   have[H0[k mrg]]:=split_self H.
-  have[H1'[H2'[x'[y'[wrx'[wr'[pd[mrg'[rd1 rd2]]]]]]]]]:=ptr_srX wrx wr mrg st.
+  have[H1'[H2'[x'[y'[wrx'[wr'[pd[mrg'[rd1 rd2]]]]]]]]]:=heap_srX wrx wr mrg st.
   have k':=pad_key pd k.
   have e:=merge_pureR mrg' k'. subst.
   exists x'. exists y'...
